---
comments: true
difficulty: Medium
edit_url: https://github.com/doocs/leetcode/edit/main/solution/3200-3299/3284.Sum%20of%20Consecutive%20Subarrays/README_EN.md
tags:
    - Array
    - Two Pointers
    - Dynamic Programming
---

<!-- problem:start -->

# [3284. Sum of Consecutive Subarrays ðŸ”’](https://leetcode.com/problems/sum-of-consecutive-subarrays)

[ä¸­æ–‡æ–‡æ¡£](/solution/3200-3299/3284.Sum%20of%20Consecutive%20Subarrays/README.md)

## Description

<!-- description:start -->

<p>We call an array <code>arr</code> of length <code>n</code> <strong>consecutive</strong> if one of the following holds:</p>

<ul>
	<li><code>arr[i] - arr[i - 1] == 1</code> for <em>all</em> <code>1 &lt;= i &lt; n</code>.</li>
	<li><code>arr[i] - arr[i - 1] == -1</code> for <em>all</em> <code>1 &lt;= i &lt; n</code>.</li>
</ul>

<p>The <strong>value</strong> of an array is the sum of its elements.</p>

<p>For example, <code>[3, 4, 5]</code> is a consecutive array of value 12 and <code>[9, 8]</code> is another of value 17. While <code>[3, 4, 3]</code> and <code>[8, 6]</code> are not consecutive.</p>

<p>Given an array of integers <code>nums</code>, return the <em>sum</em> of the <strong>values</strong> of all <strong>consecutive </strong><span data-keyword="subarray-nonempty">subarrays</span>.</p>

<p>Since the answer may be very large, return it <strong>modulo</strong> <code>10<sup>9 </sup>+ 7.</code></p>

<p><strong>Note</strong> that an array of length 1 is also considered consecutive.</p>

<p>&nbsp;</p>
<p><strong class="example">Example 1:</strong></p>

<div class="example-block">
<p><strong>Input:</strong> <span class="example-io">nums = [1,2,3]</span></p>

<p><strong>Output:</strong> <span class="example-io">20</span></p>

<p><strong>Explanation:</strong></p>

<p>The consecutive subarrays are: <code>[1]</code>, <code>[2]</code>, <code>[3]</code>, <code>[1, 2]</code>, <code>[2, 3]</code>, <code>[1, 2, 3]</code>.<br />
Sum of their values would be: <code>1 + 2 + 3 + 3 + 5 + 6 = 20</code>.</p>
</div>

<p><strong class="example">Example 2:</strong></p>

<div class="example-block">
<p><strong>Input:</strong> <span class="example-io">nums = [1,3,5,7]</span></p>

<p><strong>Output:</strong> <span class="example-io">16</span></p>

<p><strong>Explanation:</strong></p>

<p>The consecutive subarrays are: <code>[1]</code>, <code>[3]</code>, <code>[5]</code>, <code>[7]</code>.<br />
Sum of their values would be: <code>1 + 3 + 5 + 7 = 16</code>.</p>
</div>

<p><strong class="example">Example 3:</strong></p>

<div class="example-block">
<p><strong>Input:</strong> <span class="example-io">nums = [7,6,1,2]</span></p>

<p><strong>Output:</strong> <span class="example-io">32</span></p>

<p><strong>Explanation:</strong></p>

<p>The consecutive subarrays are: <code>[7]</code>, <code>[6]</code>, <code>[1]</code>, <code>[2]</code>, <code>[7, 6]</code>, <code>[1, 2]</code>.<br />
Sum of their values would be: <code>7 + 6 + 1 + 2 + 13 + 3 = 32</code>.</p>
</div>

<p>&nbsp;</p>
<p><strong>Constraints:</strong></p>

<ul>
	<li><code>1 &lt;= nums.length &lt;= 10<sup>5</sup></code></li>
	<li><code>1 &lt;= nums[i] &lt;= 10<sup>5</sup></code></li>
</ul>

<!-- description:end -->

## Solutions

<!-- solution:start -->

### Solution 1: Recurrence

We define two variables $f$ and $g$, representing the length of the increasing subarray ending at the current element and the length of the decreasing subarray ending at the current element, respectively. We use two other variables $s$ and $t$ to represent the sum of the increasing subarray ending at the current element and the sum of the decreasing subarray ending at the current element, respectively. Initially, $f = g = 1$, and $s = t = \textit{nums}[0]$.

Next, we traverse the array starting from the second element. For the current element $\textit{nums}[i]$, we consider the increasing subarray and the decreasing subarray ending at $\textit{nums}[i]$.

If $\textit{nums}[i] - \textit{nums}[i - 1] = 1$, then $\textit{nums}[i]$ can be added to the increasing subarray ending at $\textit{nums}[i - 1]$. In this case, we update $f$ and $s$, and add $s$ to the answer.

If $\textit{nums}[i] - \textit{nums}[i - 1] = -1$, then $\textit{nums}[i]$ can be added to the decreasing subarray ending at $\textit{nums}[i - 1]$. In this case, we update $g$ and $t$, and add $t$ to the answer.

Otherwise, $\textit{nums}[i]$ cannot be added to the increasing or decreasing subarray ending at $\textit{nums}[i - 1]$. We add $\textit{nums}[i]$ to the answer.

After the traversal, return the answer.

The time complexity is $O(n)$, where $n$ is the length of the array. The space complexity is $O(1)$.

<!-- tabs:start -->

#### Python3

```python
class Solution:
    def getSum(self, nums: List[int]) -> int:
        mod = 10**9 + 7
        f = g = 1
        s = t = nums[0]
        ans = nums[0]
        for x, y in pairwise(nums):
            if y - x == 1:
                f += 1
                s += f * y
                ans = (ans + s) % mod
            else:
                f = 1
                s = y
            if y - x == -1:
                g += 1
                t += g * y
                ans = (ans + t) % mod
            else:
                g = 1
                t = y
            if abs(y - x) != 1:
                ans = (ans + y) % mod
        return ans
```

#### Java

```java
class Solution {
    public int getSum(int[] nums) {
        final int mod = (int) 1e9 + 7;
        long s = nums[0], t = nums[0], ans = nums[0];
        int f = 1, g = 1;
        for (int i = 1; i < nums.length; ++i) {
            int x = nums[i - 1], y = nums[i];
            if (y - x == 1) {
                ++f;
                s += 1L * f * y;
                ans = (ans + s) % mod;
            } else {
                f = 1;
                s = y;
            }
            if (y - x == -1) {
                ++g;
                t += 1L * g * y;
                ans = (ans + t) % mod;
            } else {
                g = 1;
                t = y;
            }
            if (Math.abs(y - x) != 1) {
                ans = (ans + y) % mod;
            }
        }
        return (int) ans;
    }
}
```

#### C++

```cpp
class Solution {
public:
    int getSum(vector<int>& nums) {
        const int mod = 1e9 + 7;
        long long s = nums[0], t = nums[0], ans = nums[0];
        int f = 1, g = 1;
        for (int i = 1; i < nums.size(); ++i) {
            int x = nums[i - 1], y = nums[i];
            if (y - x == 1) {
                ++f;
                s += 1LL * f * y;
                ans = (ans + s) % mod;
            } else {
                f = 1;
                s = y;
            }
            if (y - x == -1) {
                ++g;
                t += 1LL * g * y;
                ans = (ans + t) % mod;
            } else {
                g = 1;
                t = y;
            }
            if (abs(y - x) != 1) {
                ans = (ans + y) % mod;
            }
        }
        return ans;
    }
};
```

#### Go

```go
func getSum(nums []int) int {
	const mod int = 1e9 + 7
	f, g := 1, 1
	s, t := nums[0], nums[0]
	ans := nums[0]

	for i := 1; i < len(nums); i++ {
		x, y := nums[i-1], nums[i]

		if y-x == 1 {
			f++
			s += f * y
			ans = (ans + s) % mod
		} else {
			f = 1
			s = y
		}

		if y-x == -1 {
			g++
			t += g * y
			ans = (ans + t) % mod
		} else {
			g = 1
			t = y
		}

		if abs(y-x) != 1 {
			ans = (ans + y) % mod
		}
	}

	return ans
}

func abs(x int) int {
	if x < 0 {
		return -x
	}
	return x
}
```

#### TypeScript

```ts
function getSum(nums: number[]): number {
    const mod = 10 ** 9 + 7;
    let f = 1,
        g = 1;
    let s = nums[0],
        t = nums[0];
    let ans = nums[0];

    for (let i = 1; i < nums.length; i++) {
        const x = nums[i - 1];
        const y = nums[i];

        if (y - x === 1) {
            f++;
            s += f * y;
            ans = (ans + s) % mod;
        } else {
            f = 1;
            s = y;
        }

        if (y - x === -1) {
            g++;
            t += g * y;
            ans = (ans + t) % mod;
        } else {
            g = 1;
            t = y;
        }

        if (Math.abs(y - x) !== 1) {
            ans = (ans + y) % mod;
        }
    }

    return ans;
}
```

<!-- tabs:end -->

<!-- solution:end -->

<!-- problem:end -->
